Example_Parnas_Information_Hiding_Changeable.v
@@ -4,18 +4,35 @@ Require Export Example_Parnas_Information_Hiding.
 Require Export BoehmTactics.
 
 Definition corpusChangeActionSpec (trigger: kwicAssertion) (agent: kwicStakeholders) (pre post: kwicSystemState): Prop  :=  
-        agent = customer /\ corpusPre pre /\ inMaintenancePhase pre ->
-        corpusPost post /\ satisfiesModularity_wrt corpus pre.
+        trigger = corpusPreState /\ agent = customer /\ corpusPre pre /\ inMaintenancePhase pre ->
+        corpusPost post /\ modulesChanged (value post) <= modulesChanged (value pre) + 1.
 
 Theorem verifyChangeCorpus: ActionSatisfiesActionSpec (corpusChangeActionSpec corpusPre customer) costomerChangeCorpus.
 Proof.
-Admitted.
+unfold ActionSatisfiesActionSpec.
+intros.
+unfold corpusChangeActionSpec.
+intuition.
+unfold corpusPost;auto.
+Qed.
+
+Ltac des_inv b H := destruct b; inversion H; intuition. 
+
+Theorem kwic_modularity_certificate : modular kwic_ds.
+  Proof.
+    unfold modular.
+    split.
+    unfold no_circular_satisfaction. intuition.
+    simpl in *. destruct a; try inversion H; des_inv b H. 
+    unfold no_cross_module_circular_use. split. intuition.
+    simpl in *. destruct a; try inversion H. destruct b; inversion H0. 
+    Admitted.
 
 Definition kwic_changeability_reqs (c: kwicContexts) (p: kwicPhases) (s: kwicStakeholders) (st: kwicSystemState): Prop :=
-  match c, p, s, st with
+  isModular st /\ (match c, p, s, st with
        | nominal, maintenance, customer, _ =>  ActionSatisfiesActionSpec (corpusChangeActionSpec corpusPre customer) costomerChangeCorpus
        | _, _, _, _ => True
-  end.
+  end).
 
 Definition kwic_accuracy_reqs (c: kwicContexts) (p: kwicPhases) (s: kwicStakeholders) (st: kwicSystemState): Prop := True.
 Definition kwic_physicalCapability_reqs (c: kwicContexts) (p: kwicPhases) (s: kwicStakeholders) (st: kwicSystemState): Prop := True.
@@ -72,8 +89,10 @@ Proofs for satisfying ility requirements.
 
 Theorem kwic_changeability_certificate: @Changeable kwicSystemType.
 Proof.
-Prove_satisfaction kwic_changeability_reqs c p s
-;simpl; exact verifyChangeCorpus.
+  constructor. exists kwic_changeability_reqs. intros. constructor.
+  unfold isModular. destruct (kwic_design (artifact st)). rewrite e. simpl. exact kwic_modularity_certificate. 
+  destruct c, p, st; auto.
+  simpl. destruct s; auto. exact verifyChangeCorpus.
 Qed.
 
 Theorem kwic_accuracy_certificate: @Accurate kwicSystemType.
